almost done with Show instances for all of Jasmin

proofs/progs/print_rocq_ir.v
@@ -1,8 +1,12 @@
+From Jasmin Require Export global pseudo_operator sopn expr.
 From Jasmin Require Export oracles.
 Require Export mathcomp.ssreflect.seq.
 
 (** NOTE: This should export [Show] for lists? *)
 Require Import QuickChick.QuickChick.
+
+(** [QCDerive] emits these warnings for non-recursive data types. *)
+Local Set Warnings "-non-recursive".
 
 (*** Print Rocq IR *)
 
@@ -11,19 +15,34 @@ Require Import QuickChick.QuickChick.
 (* Fail QCDerive Show for _uprog. *)
 (* Error: Anomaly "Uncaught exception Failure("destIndRef")." Please report at http://rocq-prover.org/bugs/. *)
 
+(** * Axioms for Opaque types *)
+
+Axiom show_ident : Show Ident.ident.
+Existing Instance show_ident.
+
+Axiom show_var_info : Show var_info.
+Existing Instance show_var_info.
+
+(** NOTE: I am using [funname], not [FunName.t], because
+    at extraction only [funname] is used/visible.
+
+    TODO: for what other opaque types does this apply to? *)
+Axiom show_funname : Show funname.
+Existing Instance show_funname.
+
+(** * Show Instances *)
+
+(* TODO: organize by auto-generated and manually-written instances. *)
+
 QCDerive Show for wsize.
 QCDerive Show for positive.
 QCDerive Show for atype.
-Axiom show_ident : Show Ident.ident.
-Existing Instance show_ident.
 Instance show_var : Show var :=
   {| show (x : var) :=
       match x with
       | {| vtype := p0; vname := p1 |} =>
           ("Var " ++ smart_paren (show p0) ++ " " ++ smart_paren (show p1))%string
       end |}.
-Axiom show_var_info : Show var_info.
-Existing Instance show_var_info.
 Instance show_var_i : Show var_i :=
   {| show (x : var_i) :=
        match x with
@@ -50,6 +69,16 @@ QCDerive Show for sop2.
 QCDerive Show for pelem.
 QCDerive Show for combine_flags.
 QCDerive Show for opN.
+
+Print word.
+
+(* QCDerive Show for word.word.word. *)
+
+(* QCDerive Show for WArray.array. *)
+
+(* QCDerive Show for word. *)
+
+(* QCDerive Show for glob_value.  *)
 
 (* But [Show] does exist for [list] ... *)
 Fail QCDerive Show for pexpr.
@@ -84,3 +113,218 @@ Fixpoint show_pexpr_aux (e : pexpr) : string :=
   | PappN op es => "PappN " ++ smart_paren (show op) ++ " " ++ show__list show_pexpr_aux es
   | Pif t e e1 e2 => show0 ("Pif" :: map smart_paren [:: show t; show_pexpr_aux e; show_pexpr_aux e1; show_pexpr_aux e2])
   end%string.
+
+Global Instance show_pexpr : Show pexpr :=
+  {| show := show_pexpr_aux |}.
+
+QCDerive Show for opN_safety.
+QCDerive Show for eassert.
+
+Global Instance show_lval : Show lval :=
+  {| show lv :=
+      match lv with
+      | Lnone p0 p1 =>
+          ("Lnone " ++ smart_paren (show p0) ++ " " ++ smart_paren (show p1))%string
+      | Lvar p0 => ("Lvar " ++ smart_paren (show p0))%string
+      | Lmem p0 p1 p2 p3 =>
+          ("Lmem " ++
+             smart_paren (show p0) ++
+             " " ++
+             smart_paren (show p1) ++
+             " " ++ smart_paren (show p2) ++ " " ++ smart_paren (show p3))%string
+      | Laset p0 p1 p2 p3 p4 =>
+          ("Laset " ++
+             smart_paren (show p0) ++
+             " " ++
+             smart_paren (show p1) ++
+             " " ++
+             smart_paren (show p2) ++
+             " " ++ smart_paren (show p3) ++ " " ++ smart_paren (show p4))%string
+      | Lasub p0 p1 p2 p3 p4 =>
+          ("Lasub " ++
+             smart_paren (show p0) ++
+             " " ++
+             smart_paren (show p1) ++
+             " " ++
+             smart_paren (show p2) ++
+             " " ++ smart_paren (show p3) ++ " " ++ smart_paren (show p4))%string
+      end |}.
+
+QCDerive Show for spill_op.
+QCDerive Show for pseudo_operator.
+QCDerive Show for slh_op.
+
+Global Instance show_prim_x86_suffix : Show prim_x86_suffix :=
+  {| show x :=
+      match x with
+      | PVp p0 => ("PVp " ++ smart_paren (show p0))%string
+      | PVs p0 p1 => ("PVs " ++ smart_paren (show p0) ++ " " ++ smart_paren (show p1))%string
+      | PVv p0 p1 => ("PVv " ++ smart_paren (show p0) ++ " " ++ smart_paren (show p1))%string
+      | PVsv p0 p1 p2 =>
+          ("PVsv " ++
+             smart_paren (show p0) ++
+             " " ++ smart_paren (show p1) ++ " " ++ smart_paren (show p2))%string
+      | PVx p0 p1 => ("PVx " ++ smart_paren (show p0) ++ " " ++ smart_paren (show p1))%string
+      | PVvv p0 p1 p2 p3 =>
+          ("PVvv " ++
+             smart_paren (show p0) ++
+             " " ++
+             smart_paren (show p1) ++
+             " " ++ smart_paren (show p2) ++ " " ++ smart_paren (show p3))%string
+      end |}.
+
+(* Error: Case Not Handled *)
+Fail QCDerive Show for prim_constructor.
+
+(* Error: *)
+(* Anomaly *)
+(* "Uncaught exception Failure("Not a valid class name. Expected one of : GenSized , EnumSized , Shrink , Arbitrary , Show , Sized , DecOpt , ArbitrarySizedSuchThat , GenSizedSuchThat , EnumSizedSuchThat , Generator , Enumerator , Checker")." *)
+(* Please report at http://rocq-prover.org/bugs/. *)
+(* Fail QCDerive ShowFunctions.ReprSubset for prim_x86_suffix. *)
+
+(* TODO: *)
+Global Instance repr_prim_x86_suffix : ShowFunctions.ReprSubset prim_x86_suffix :=
+  {| ShowFunctions.representatives := [::] |}.
+
+Global Instance show_result {E A : Type} `{Show E, Show A} : Show (result E A) :=
+  {| show r :=
+      match r with
+      | Ok _ x => "Ok " ++ smart_paren (show x)
+      | Error x => "Error " ++ smart_paren (show x)
+      end%string |}.
+
+Global Instance show_prim_constructor {asm_op : Type} `{!Show asm_op}
+  : Show (prim_constructor asm_op) :=
+  {| show pc :=
+      match pc with
+      | PrimX86 prim_suffixes prim_suffix_fun =>
+          "PrimX86 " ++ smart_paren (show prim_suffixes) ++ " " ++ smart_paren (show prim_suffix_fun)
+      | PrimARM f =>
+          "PrimARM " ++ smart_paren (show f)
+      end%string |}.
+
+QCDerive Show for assgn_tag.
+QCDerive Show for syscall_t.
+QCDerive Show for dir.
+
+(* Error: Anomaly "Uncaught exception Failure("destIndRef")." *)
+(* Please report at http://rocq-prover.org/bugs/. *)
+(* Fail QCDerive Show for range. *)
+
+(* FIXME: why doesn't [showPair] just work with this automatically? *)
+Global Instance show_range : Show range :=
+  {| show r := show r |}.
+
+(* Bruh? *)
+Fail QCDerive Show for align.
+
+Global Instance show_align : Show align :=
+  {| show a :=
+      match a with
+      | Align => "Align"
+      | NoAlign => "NoAlign"
+      end%string |}.
+
+Section ASM_OP.
+  Context {asm_op : Type} `{asmop : !asmOp asm_op}.
+
+  (* TODO: is this correct? *)
+  Context `{show_asm_op : !Show asm_op}.
+
+  (* TODO: Do I need this? Because of the [asm_op_t] wrapper? *)
+  (* Global Instance show_asm_op_t : Show asm_op_t := show_asm_op. *)
+
+  Fail QCDerive Show for sopn.
+
+  Global Instance show_sopn : Show sopn :=
+    {| show o :=
+        match o with
+        | Opseudo_op o => "Opseudo_op " ++ smart_paren (show o)
+        | Oslh o => "Oslh " ++ smart_paren (show o)
+        | Oasm o => "Oasm " ++ smart_paren (show o)
+        end%string |}.
+
+(* Error: *)
+(* In environment *)
+(* asm_op : Type *)
+(* asmop : asmOp asm_op *)
+(* show_asm_op : Show asm_op *)
+(* asm_op0 : Type *)
+(* H : Show asm_op0 *)
+(* asmop0 : Type *)
+(* H0 : Show asmop0 *)
+(* The term "asmop0" has type "Type" while it is expected to have type "asmOp asm_op0". *)
+  Fail QCDerive Show for instr_r.
+
+  Fixpoint show_instr_r_aux (i : instr_r) : string :=
+    match i with
+    | Cassgn lv tg t e =>
+        show0 ("Cassgn" :: map smart_paren [:: show lv; show tg; show t; show e])
+    | Copn lvs tg o es =>
+        show0 ("Copn" :: map smart_paren [:: show lvs; show tg; show o; show es])
+    | Csyscall lvs o es =>
+        show0 ("Csyscall" :: map smart_paren [:: show lvs; show o; show es])
+    | Cassert a => "Cassert " ++ smart_paren (show a)
+    | Cif e c1 c2 =>
+        show0 [:: "Cif"; smart_paren (show e); show__list show_instr_aux c1;  show__list show_instr_aux c2]
+    | Cfor x r c =>
+        show0 ("Cfor" :: map smart_paren [:: show x; show r] ++ [:: show__list show_instr_aux c])
+    | Cwhile a c e ii c' =>
+        (* NOTE: for now, throw away info *)
+        show0 [:: "Cwhile"; smart_paren (show a); show__list show_instr_aux c; smart_paren (show e); show__list show_instr_aux c']
+    | Ccall lvs f es =>
+        show0 [:: "Ccall"; show lvs; show f; show es]
+    end%string
+  (* NOTE: for now, throwing away instruction info.
+     Should I care about this?
+     It just seems like noise... *)
+  with show_instr_aux (i : instr) : string :=
+         match i with
+         | MkI _ i => show_instr_r_aux i
+         end.
+
+  Global Instance show_instr_r : Show instr_r :=
+    {| show := show_instr_r_aux |}.
+
+  Global Instance show_instr : Show instr :=
+    {| show := show_instr_aux |}.
+
+  Global Instance show_fun_contract : Show fun_contract :=
+    {| show x :=
+        match x with
+        | {| f_iparams := p0; f_ires := p1; f_pre := p2; f_post := p3 |} =>
+            ("MkContra " ++
+               smart_paren (show p0) ++
+               " " ++
+               smart_paren (show p1) ++
+               " " ++ smart_paren (show p2) ++ " " ++ smart_paren (show p3))%string
+        end |}.
+
+  Section extra_fun_t.
+    Context `{!progT}.
+    Context `{!Show extra_fun_t, !Show extra_prog_t, !Show extra_val_t}.
+
+    Global Instance show_fundef : Show fundef :=
+      {| show fd :=
+          (* NOTE: ignoring [fun_info] for now. *)
+          show0 ("MkFun"%string :: map smart_paren
+                   [:: show fd.(f_contract);
+                    show fd.(f_tyin);
+                    show fd.(f_params);
+                    show fd.(f_body);
+                    show fd.(f_tyout);
+                    show fd.(f_res);
+                    show fd.(f_extra)]) |}.
+
+    (* Fail QCDerive Show for fun_decl. *)
+    Global Instance show_fun_decl : Show fun_decl :=
+      {| show fd := show fd |}.
+
+    Fail Global Instance show_prog : Show prog :=
+      {| show p :=
+          show0 ("Build__prog"%string :: map smart_paren
+                   [:: show p.(p_funcs);
+                    show p.(p_globs);
+                    show p.(p_extra)]) |}.
+  End extra_fun_t.
+End ASM_OP.
